LEProps3.v
@@ -71,7 +71,7 @@ Inductive value_has_type : evalue -> ty -> Prop :=
 with rtcontext_has_type: rctx -> context -> Prop :=
   | TC_nil : nil :::* empty
   | TC_cons : forall G g x v T, 
-                g :::* G -> v ::: T -> (aextend x v g) :::* extend G x T
+                g :::* G -> v ::: T -> (aextend x v g) :::* add_vdecl x T G
 
 with evaluates_to_a : tm -> rctx ->  ty -> Prop := 
    | TVE : forall t g T,  
@@ -113,7 +113,7 @@ Lemma ctxts_agree_on_lookup :
 Proof.
   introv Hctxts HGxT. induction Hctxts.
     Case "TC_nil". inversion HGxT.
-    Case "TC_cons". unfold lookup_vdecl, extend in HGxT. 
+    Case "TC_cons". unfold lookup_vdecl, add_vdecl in HGxT. 
     destruct (eq_id_dec x0 x).
       SCase "x0=x". subst. inverts HGxT. exists v. split.
         simpl. apply eq_id.
